Bakery/DMC.lean
@@ -1,0 +1,97 @@
+import Mathlib.Logic.Relation
+
+class IndInv (Conf : Type) (inv : Conf → Prop)
+  (init : Conf → Prop) (step : Conf → Conf → Prop) where
+    base : ∀ cf : Conf, init cf → inv cf
+    ind : ∀ (cf cf' : Conf), (inv cf ∧ (step cf cf')) → (inv cf')
+
+variable {Conf : Type}
+variable {inv init : Conf → Prop}
+variable {step : Conf → Conf → Prop}
+
+theorem invariant
+    [hInv : IndInv Conf inv init step]
+    {cf cf' : Conf}
+    (h0 : init cf)
+    (hrt : Relation.ReflTransGen step cf cf') :
+    inv cf' := by
+  induction hrt with
+  | refl =>
+      -- this case is cf' = cf
+      -- so we just use base
+      have : inv cf := hInv.base cf h0
+      -- x is definitionaly cf, so:
+      simpa using this
+  | tail hxy hyz ih =>
+      -- hxy : ReflTransGen step cf ?y
+      -- hyz : step ?y ?z
+      -- ih  : pred ?y
+      have hpair : inv _ ∧ step _ _ := ⟨ih, hyz⟩
+      exact hInv.ind _ _ hpair
+
+-- --- Conjunction of invariants is an invariant
+-- instance IndInvConj
+--     (pred₁ pred₂ init step)
+--     [h1 : IndInv pred₁ init step]
+--     [h2 : IndInv pred₂ init step] :
+--     IndInv (fun cf => pred₁ cf ∧ pred₂ cf) init step where
+--   base cf h0 :=
+--     ⟨h1.base cf h0, h2.base cf h0⟩
+--   ind cf cf' h := by
+--     rcases h with ⟨⟨hp1, hp2⟩, hstep⟩
+--     exact ⟨h1.ind cf cf' ⟨hp1, hstep⟩, h2.ind cf cf' ⟨hp2, hstep⟩⟩
+
+--- “Safety” meta-theorem: no bad state is reachable
+def Safe (init : Conf → Prop) (step : Conf → Conf → Prop) (Bad : Conf → Prop) : Prop :=
+  ∀ cf cf', init cf → Relation.ReflTransGen step cf cf' → ¬ Bad cf'
+
+theorem IndInv.safe
+    {inv init safe_pred : Conf → Prop} {step : Conf → Conf → Prop}
+    [IndInv Conf inv init step]
+    (invSafe : ∀ cf, inv cf → safe_pred cf) :
+    ∀ cf cf', init cf → Relation.ReflTransGen step cf cf' → safe_pred cf' := by
+  intro cf cf' h0 hreach
+  -- from inductive invariant:
+  have hp : inv cf' :=
+    invariant (inv:=inv) (init:=init) (step:=step) h0 hreach
+  exact invSafe cf' hp
+
+
+theorem IndInv.safe1
+    {inv init : Conf → Prop} {step : Conf → Conf → Prop}
+    [IndInv Conf inv init step]
+    (Bad : Conf → Prop)
+    (hExclude : ∀ cf, inv cf → ¬ Bad cf) :
+    Safe init step Bad := by
+  intro cf cf' h0 hreach
+  -- from inductive invariant:
+  have hp : inv cf' :=
+    invariant (inv:=inv) (init:=init) (step:=step) h0 hreach
+  exact hExclude cf' hp
+
+
+-- --- Restricting the initial set
+-- theorem IndInv.restrict_init
+--     {pred init init' : Conf → Prop} {step : Conf → Conf → Prop}
+--     [hInv : IndInv pred init step]
+--     (hSub : ∀ cf, init' cf → init cf) :
+--     IndInv pred init' step where
+--   base cf h0 :=
+--     hInv.base cf (hSub cf h0)
+--   ind cf cf' h :=
+--     hInv.ind cf cf' h
+
+-- --- Invariants for an equivalent step relation
+-- theorem IndInv.congr_step
+--     {pred init : Conf → Prop}
+--     {step₁ step₂ : Conf → Conf → Prop}
+--     (hEq : ∀ cf cf', step₁ cf cf' ↔ step₂ cf cf')
+--     [hInv : IndInv pred init step₁] :
+--     IndInv pred init step₂ where
+--   base cf h0 := hInv.base cf h0
+--   ind cf cf' h := by
+--     -- h : pred cf ∧ step₂ cf cf'
+--     have h' : pred cf ∧ step₁ cf cf' :=
+--       ⟨h.1, (hEq cf cf').mpr h.2⟩
+--     -- reuse old instance
+--     exact hInv.ind cf cf' h'
